added proper handling for environment in generic extraction

theories/GenExtract/GenExtractPCF.v
@@ -43,13 +43,13 @@ Module Env.
     | S m => fun xs => (f (fst xs),map__V f (snd xs))
     end.
 
-  (*
-  Lemma cast_nthV_mapV {n} {X Y} (f : X -> Y) i (vs : vec X n):
+  
+  Lemma nthV_mapV {n} {X Y} (f : X -> Y) i (vs : vec X n):
     nth__V i (map__V f vs) = f (nth__V i vs).
   Proof.
     induction n;cbn in *. easy.
     destruct i;cbn in *. all:easy.
-  Qed. *)
+  Qed.
 
   
 End Env.
@@ -126,8 +126,8 @@ Inductive isPCF : forall n (Γ : typeContext n) (A: anyTT), (valueContext Γ -> 
 | isPCF_Succ n Γ:
     @isPCF n Γ (TyArr _ _) (fun _ => S)
 | isPCF_Fix_unaryNat n Γ (A:anyTT) f (F : valueContext Γ -> nat -> A.(aTy))
-                     (H__Fix : forall (ctx : valueContext Γ) (x:nat), F ctx x = f (x,(F ctx,ctx))) :
-    isPCF (S (S n)) ({|aTT := TyNat|},({|aTT := TyArr TyNat A|},Γ)) A f
+                     (H__Fix : forall (ctx : valueContext Γ) (x:nat), F ctx x = f ctx (F ctx) x) :
+    isPCF n Γ (TyArr (TyArr TyNat A) (TyArr TyNat A)) f
     -> isPCF n Γ {|aTT := TyArr TyNat A|} (fun ctx x => F ctx x).
 
 Arguments isPCF_Const {n Γ} c.
@@ -148,11 +148,13 @@ Lemma isPCF_plus n (Γ: typeContext n): isPCF Γ (TyArr _ (TyArr _ _)) (fun _ =>
 Proof.
   unfold Init.Nat.add.
   apply @isPCF_Fix_unaryNat with (A := {| aTT := (TyArr TyNat TyNat) |} )
-                                 (f:= fun ctx=> fun m => match fst ctx with
+                                 (f:= fun ctx=> fun F n m => match n  with
                                                    | 0 => m
-                                                   | S p => S (fst (snd ctx) p m)
+                                                   | S p => S (F p m)
                                                    end).
   now intros arg [].
+  eapply @isPCF_Lambda with (A := (TyNat ~> TyNat ~> TyNat)) (B := (TyNat ~> TyNat ~> TyNat)).
+  eapply @isPCF_Lambda with (A := TyNat) (B := (TyNat ~> TyNat)).
   eapply @isPCF_Lambda with (A := TyNat) (B := TyNat).
   simple eapply @isPCF_Case_nat.
   -eapply @isPCF_Rel with (x:=Some None).
@@ -169,20 +171,20 @@ Defined.
 From Undecidability Require Import LNat.
 
 
-Local Notation "↑ env" := (0,map__V S env) (at level 10).
+Definition up {n} (env : vec nat n) := (0,map__V S env).
 
 Fixpoint PCFtoL {n} {Γ : typeContext n} {A:anyTT} {f:valueContext Γ -> A.(aTy)} (H : isPCF Γ A f): vec nat n -> term :=
   match H with
   | @isPCF_Const n Γ c => fun ren => enc c
   | @isPCF_Rel n Γ x =>  fun ren => var (nth__V x ren)
   | @isPCF_App n Γ A B f arg H__f H__arg =>  fun ren => app (PCFtoL H__f ren) (PCFtoL H__arg ren)
-  | @isPCF_Lambda n Γ A B f H__f =>  fun ren => lam (PCFtoL H__f (↑ ren))
+  | @isPCF_Lambda n Γ A B f H__f =>  fun ren => lam (PCFtoL H__f (up ren))
 
   (* TODO: lambda-lift for "lazy" evaluation?*)
   | @isPCF_Case_nat n Γ A x f__O f__S H__x H__O H__S =>  fun ren => app (app (PCFtoL H__x ren) (PCFtoL H__O ren)) (PCFtoL H__S ren)
                                                   
   | @isPCF_Succ n Γ =>  fun ren => ext S
-  | @isPCF_Fix_unaryNat n Γ A f F H__Fix H__F =>  fun ren => rho (lam (lam (PCFtoL H__F (0,(1,map__V S ren)))))
+  | @isPCF_Fix_unaryNat n Γ A f F H__Fix H__F =>  fun ren => rho ((PCFtoL H__F (map__V S ren)))
   end.
 
 Fixpoint vec_to_list {n X} : vec X n -> list X :=
@@ -191,13 +193,41 @@ Fixpoint vec_to_list {n X} : vec X n -> list X :=
   | S n => fun xs => fst xs :: vec_to_list (snd xs)
   end.
 
-Lemma In_vec_to_list {X n} (x:X) (v:vec X n):
+Lemma vec_to_list_In {X n} (x:X) (v:vec X n):
   In x (vec_to_list v) -> exists i, nth__V i v = x.
 Proof.
   induction n;cbn in *. easy. intros [ <- | ]. now eexists None.
   edestruct IHn as [i ?]. eauto. now eexists (Some i).
 Qed.
 
+Lemma vec_to_list_length {n X} (xs : vec X n):
+  length (vec_to_list xs) = n.
+Proof. induction n in xs |-*;cbn. easy. now rewrite IHn. Qed.
+
+Fixpoint nat_to_fin {n i} : i < n -> fin n.
+  refine (match n with
+            0 => fun H => False_rect _ _
+          | S n => match i as i return i < (S n) -> fin (S n) with
+                    0 => fun _ => None
+                  | S i => fun H => Some (@nat_to_fin n i _)
+                  end
+          end).
+  all:abstract nia.
+Defined.
+
+Lemma nat_to_fin_unique {n i} (H1 H2 : i < n) :
+  nat_to_fin H1 = nat_to_fin H2.
+Proof.
+  unfold lt in *. replace H2 with H1. easy. apply le_unique.
+Qed.
+
+
+Lemma vec_to_list_nth n X (vs:vec X n) i (H : i < n) d:
+  nth i (vec_to_list vs) d = nth__V (nat_to_fin H) vs.
+Proof.
+  induction n in vs,i,H |-*. nia. destruct vs. cbn.
+  destruct i. easy. erewrite IHn. reflexivity.
+Qed.
 
 Lemma extensionalMatch_nat {X} (T : X -> Type) n H__O H__S:
   T (match n with 0 => H__O | S n => H__S n end) = match n with 0 => T H__O | S n => T (H__S n) end.
@@ -219,36 +249,78 @@ Proof.
   now intros ? ? [].
 Defined.
 
-
-Lemma isPCP_L_computable {n} {Γ : typeContext n} {A:anyTT} {f:valueContext Γ -> A.(aTy)}
-      (H : isPCF Γ A f) (vs : valueContext Γ) (env__L : vec term n) (ren : vec nat n) :
-  hvec proc env__L ->
-  {v & (LClos.substList (PCFtoL H ren) 0 (vec_to_list env__L) >* v) * computes A.(aTT) (f vs) v}%type.
+Lemma substList_rho s k A:
+  LClos.substList (rho s) k A = rho (LClos.substList s (S k) A).
 Proof.
-  induction H;intros proc__env.
+  reflexivity.
+Qed.
+
+Lemma validEnv'_vec_to_list {n} (env__L : vec _ n):
+  hvec proc env__L -> LClos.validEnv' (vec_to_list env__L).
+Proof. intros proc__env. intros ? (i&<-)%vec_to_list_In. now destruct (nth__HV i proc__env). Qed.
+
+Lemma hvec_map {X Y} {P} (f:X -> Y) {n} (xs : vec X n): 
+  hvec P (map__V f xs) = hvec (fun x => P (f x)) xs.
+Proof. induction n in xs|-*;cbn. easy. rewrite IHn.  reflexivity. Qed.
+
+Lemma hvec_impl {X} {P Q} {n} (xs : vec X n):
+  (forall x, P x -> Q x) -> hvec P xs -> hvec Q xs.
+Proof. induction n in xs|-*;cbn. easy. intros ? [];split. all:eauto. Qed.
+
+Lemma bound_PCFtoL {n} {Γ : typeContext n} {A:anyTT} {f:valueContext Γ -> A.(aTy)}
+      (H : isPCF Γ A f) (ren : vec nat n) k:
+  hvec (fun x => x < k) ren
+  -> bound k (PCFtoL H ren).
+Proof.
+  induction H in ren,k |- *;intros Hlt;cbn.
+  1,6:now apply closed_dcl_x; Lproc.
+  2,4:now repeat econstructor;eauto using bound.
+  -econstructor. hnf. eapply (nth__HV x Hlt).
+  -econstructor. eapply IHisPCF. cbn. split. easy. rewrite hvec_map. eapply hvec_impl with (2:=Hlt). nia.
+  -eapply rho_dcls. apply IHisPCF with (k:= S k). rewrite hvec_map. eapply hvec_impl with (2:=Hlt). nia.
+Qed.
+
+Lemma bound_up n d (ren : vec nat n) :
+  hvec (fun x => x < d) ren -> hvec (n:=S n) (fun x : nat => x < S d) (up ren).
+Proof. intros H. cbn. split. easy. rewrite hvec_map. eapply hvec_impl with (2:=H). nia. Qed. 
+
+Lemma isPCF_L_computable {n} {Γ : typeContext n} {A:anyTT} {f:valueContext Γ -> A.(aTy)}
+      (H : isPCF Γ A f) (vs : valueContext Γ) k (env__L : vec term k) (ren : vec nat n) 
+      (proc__env  : hvec proc env__L) (bound__ren : hvec (fun x => x < k) ren):
+  (forall i, computes (nth__V i Γ).(aTT) (nth__HV i vs) (nth__V (nat_to_fin (nth__HV i bound__ren)) env__L))
+  -> {v & (LClos.substList (PCFtoL H ren) 0 (vec_to_list env__L) >* v) * computes A.(aTT) (f vs) v}%type.
+Proof.
+  revert k env__L proc__env bound__ren.
+  induction H;intros k env__L proc__env bound__ren H__env.
   1:{(* Const*) do 2 esplit. cbn. rewrite LClos.substList_closed. 1,3:reflexivity. Lproc. }
-  1:{(*Rel*) cbn. rewrite Nat.sub_0_r. do 2 esplit. reflexivity. admit. }
-  1:{(*App*) cbn. edestruct IHisPCF2  with (1:=proc__env) as (v2&R2&IH2). 
-      cbn in IHisPCF1. edestruct IHisPCF1 as (v&R&Hproc&v'&R'&IH1). 1,2:eassumption.
+  1:{(*Rel*) cbn. rewrite Nat.sub_0_r. do 2 esplit. reflexivity.
+     erewrite vec_to_list_nth. apply H__env. 
+  }
+  1:{(*App*) cbn. edestruct IHisPCF2  with (1:=proc__env) (bound__ren:=bound__ren) (2:=H__env) as (v2&R2&IH2). 
+      cbn in IHisPCF1. edestruct IHisPCF1 with (2:=H__env) as (v&R&Hproc&v'&R'&IH1) . 1,2:eassumption. 
       eexists;split. 2:easy. rewrite R,R2. easy.
   }
   1:{ (*Lambda *) cbn.
       eexists. split. reflexivity. split. split. 2:easy.
-      { (*PCFtoL is closed *) admit. }
+      { (*PCFtoL is closed *) apply closed_dcl. constructor. apply LClos.substList_is_bound.
+        1:now apply validEnv'_vec_to_list. rewrite vec_to_list_length. now  eapply bound_PCFtoL, bound_up. }
       intros.
-      edestruct IHisPCF with (vs := (a,vs)) (env__L := (t_a,env__L)) as (v&R&IH).
+      unshelve edestruct IHisPCF with (k:= S k) (vs := (a,vs)) (env__L := (t_a,env__L)) (ren := (up ren)) as (v&R&IH).
+      {now apply  bound_up. }
       {split;cbn. all:eauto using computesProc. }
-
+      {intros []. 2:assumption. cbn.
+       set (l:=nth__HV f0 (snd (bound_up _ k ren bound__ren))). cbn in l. fold l. generalize l. clear l.
+       rewrite nthV_mapV. intros ?. cbn. erewrite nat_to_fin_unique. apply H__env.
+      }
       cbn in IH.
       eexists. split. 
       rewrite step_Lproc. 2:now eapply computesProc. 2:exact IH.
-      rewrite LClos.subst_substList. eassumption.
-      { hnf. intros ? (i&<-)%In_vec_to_list. now destruct (nth__HV i proc__env). }
+      rewrite LClos.subst_substList. eassumption. now eapply validEnv'_vec_to_list.
   }
   1:{ (* Case_nat *) cbn.
-      specialize IHisPCF1 with (vs:=vs) (ren:=ren) (env__L := env__L) (1:=proc__env).
-      specialize IHisPCF2 with (vs:=vs) (ren:=ren) (env__L := env__L) (1:=proc__env).
-      specialize IHisPCF3 with (vs:=vs) (ren:=ren) (env__L := env__L) (1:=proc__env).
+      specialize IHisPCF1 with (vs:=vs) (ren:=ren) (env__L := env__L) (1:=proc__env) (bound__ren:=bound__ren) (2:=H__env).
+      specialize IHisPCF2 with (vs:=vs) (ren:=ren) (env__L := env__L) (1:=proc__env) (bound__ren:=bound__ren) (2:=H__env).
+      specialize IHisPCF3 with (vs:=vs) (ren:=ren) (env__L := env__L) (1:=proc__env) (bound__ren:=bound__ren) (2:=H__env).
 
       edestruct IHisPCF1 as (_ &R__x &[= -> ]).
       edestruct IHisPCF2 as (v__O &R__O &IH__O).
@@ -273,5 +345,15 @@ Proof.
       exact IH.
   }
   1:{(* Succ *) eexists;split. reflexivity. cbn - [computes]. rewrite LClos.substList_closed. 2:now Lproc. apply extCorrect. }
-  1:{(* Fix_unaryNat *) cbn - [rho]. admit. }
+  1:{(* Fix_unaryNat *) cbn - [rho].
+     eexists. split. reflexivity. split. split. 2:cbn;easy.
+     { (*PCFtoL is closed *) apply closed_dcl. rewrite substList_rho. apply rho_dcls, LClos.substList_is_bound.
+       1:now apply validEnv'_vec_to_list. rewrite vec_to_list_length.
+       eapply bound_PCFtoL. rewrite hvec_map. eapply hvec_impl with (2:=bound__ren). nia.
+     } 
+     intros x ? ->. eexists. split.
+     
+     set (REC := PCFtoL _ _).
+     rewrite substList_rho. rewrite rho_correct. 2:  (*PCFtoL is closed *) admit. 2:Lproc. all:admit (*TODO: recursion *). 
+  }
 Admitted.
